@prefix : <https://ontology.tno.nl/logistics/federated/BusinessActivity#> .
@prefix rdfs: <http://www.w3.org/2000/01/rdf-schema#> .
@prefix skos: <http://www.w3.org/2004/02/skos/core#> .
@prefix xsd: <http://www.w3.org/2001/XMLSchema#> .
@prefix dc: <http://purl.org/dc/elements/1.1/> .
@prefix dcterms: <http://purl.org/dc/terms/> .
@prefix owl: <http://www.w3.org/2002/07/owl#> .
@prefix Location: <https://ontology.tno.nl/logistics/federated/Location#> .
@prefix foaf: <http://xmlns.com/foaf/0.1/> .

:BusinessActivity
  a owl:Class ;
  rdfs:comment "A business activity bundles all the information associated to a business transaction" ;
  rdfs:label "Business Activity" ;
.
:UUID a owl:DatatypeProperty ;
  rdfs:comment "Every Business Activity has a UUID to identify its' relation to an event" ;
  rdfs:label "UUID" ;
  rdfs:domain :BusinessActivity ;
  rdfs:range xsd:string
.
:involvesDate
    a owl:DatatypeProperty ;
    rdfs:label "Date" ;
    rdfs:comment "Bill of lading issue date / voyage charter party date" ;
    rdfs:domain :BusinessActivity ;
    rdfs:range xsd:string ;
    owl:equivalentProperty Location:locode ;
.
:involvesLoCode 
    a owl:DatatypeProperty ;
    rdfs:label "LoCode" ;
    rdfs:comment "Bill of lading issued location, coded" ;
    rdfs:domain :BusinessActivity ;
    rdfs:range xsd:string ;
    owl:equivalentProperty Location:locode ;
.
:numberOriginal
    a owl:DatatypeProperty ;
    rdfs:label "Number Original" ;
    rdfs:comment "Number of original Bill of Ladings" ;
    rdfs:domain :BusinessActivity ;
    rdfs:range xsd:integer ;
.
:numberCopies
    a owl:DatatypeProperty ;
    rdfs:label "Number Copies" ;
    rdfs:comment "Number of Bill of Lading copies" ;
    rdfs:domain :BusinessActivity ;
    rdfs:range xsd:integer ;
.
:termsConditions
    a owl:ObjectProperty ;
    rdfs:label "Terms and Conditions" ;
    rdfs:comment "Terms and conditions in the transport document - can be expressed as plain text or a URL to the publicly accessible document itself" ;
    rdfs:domain :BusinessActivity ;
    rdfs:range xsd:integer ;
    rdfs:range foaf:Document
.
:carrierClauses
    a owl:ObjectProperty ;
    rdfs:label "Carrier Clauses" ;
    rdfs:comment "Description of additional clauses for a specific shipment added by carrier to B/L - can be expressed as plain text or a URL to a publicly accessible document" ;
    rdfs:domain :BusinessActivity ;
    rdfs:range xsd:integer ;
    rdfs:range foaf:Document
.