# baseURI: https://ontology.tno.nl/logistics/federated/Event
# imports: https://ontology.tno.nl/logistics/federated/BusinessService
# prefix: Event

@prefix : <https://ontology.tno.nl/logistics/federated/Event#> .
@prefix DigitalTwin: <https://ontology.tno.nl/logistics/federated/DigitalTwin#> .
@prefix LegalPerson: <https://ontology.tno.nl/logistics/federated/LegalPerson#> .
@prefix dc: <http://purl.org/dc/elements/1.1/> .
@prefix dcterms: <http://purl.org/dc/terms/> .
@prefix owl: <http://www.w3.org/2002/07/owl#> .
@prefix Location: <https://ontology.tno.nl/logistics/federated/Location#> .
@prefix rdfs: <http://www.w3.org/2000/01/rdf-schema#> .
@prefix skos: <http://www.w3.org/2004/02/skos/core#> .
@prefix xsd: <http://www.w3.org/2001/XMLSchema#> .

<https://ontology.tno.nl/logistics/federated/Event>
  a owl:Ontology ;
  dc:creator "Dena Tahvildari, Maaike Burghoorn, Cornelis Bouter, Theodor Chirvasuta" ;
  dcterms:created "2020-07-17" ;
  dcterms:description "This ontology contains classes, attributes, relation about logistic Events." ;
  dcterms:issued "2021-03-15" ;
  dcterms:modified "2023-07-18" ;
  dcterms:language "en" ;
  dcterms:requires <https://ontology.tno.nl/logistics/federated/LegalPerson> ;
  dcterms:requires <https://ontology.tno.nl/logistics/federated/DigitalTwin> ;
  dcterms:requires <https://ontology.tno.nl/logistics/federated/Location> ;
  owl:versionIRI <https://ontology.tno.nl/logistics/federated/Eventv-0.1> ;
.

# High level Event classes

:Event
  a owl:Class ;
  rdfs:comment "An event reflects a conceptual association of digital twins or a virtualization of a physical event" ;
  rdfs:label "Event" ;
.
:AssociationEvent
  a owl:Class ;
  rdfs:comment "Association event that may associate digital twins with business identifiers or other digital twins" ;
  rdfs:label "Association Event" ;
  rdfs:subClassOf :Event ;
.
:PrimitiveEvent
  a owl:Class ;
  rdfs:comment "A primitive event represents a virtualization of a physical event, i.e. arrival, load, discharge etc." ;
  rdfs:label "Primitive Event" ;
  rdfs:subClassOf :Event ;
.

# Unique identifier for storage of event

:UUID a owl:DatatypeProperty ;
  rdfs:comment "Every event has a UUID to be distinguishable when stored in a database." ;
  rdfs:label "UUID" ;
  rdfs:domain :Event ;
  rdfs:range xsd:string
.

# Association event classes
:BusinessAssociation
  a owl:Class ;
  rdfs:comment "Business association event that may associate digital twin(s) with a business identifier" ;
  rdfs:label "Business Association" ;
  rdfs:subClassOf :AssociationEvent ;
.
:CargoAssociation
  a owl:Class ;
  rdfs:comment "Cargo association event that may associate (dangerous) goods with a transport equipment" ;
  rdfs:label "Cargo Association" ;
  rdfs:subClassOf :AssociationEvent ;
.
:LocationAssociation
  a owl:Class ;
  rdfs:comment "Location Association may associate a legal person or a transport means to a location" ;
  rdfs:label "Location Association" ;
  rdfs:subClassOf :AssociationEvent ;
.
:TransportMeansAssociation
  a owl:Class ;
  rdfs:comment "Transport means association event that may associate cargo (goods or equipment) with a transport means" ;
  rdfs:label "Transport Means Association" ;
  rdfs:subClassOf :AssociationEvent ;
.
# Time classification

:TimeClassification a owl:Class ;
  rdfs:comment "Time classification can be either Planned, Estimated, Expected, Actual, Requested." ;
  rdfs:label "Time Classification" ;
.
:Actual
  a :TimeClassification ;
  rdfs:label "Actual" ;
.
:Estimated
  a :TimeClassification ;
  rdfs:label "Estimated" ;
.
:Expected
  a :TimeClassification ;
  rdfs:label "Expected" ;
.
:Planned
  a :TimeClassification ;
  rdfs:label "Planned" ;
.
:Requested
  a :TimeClassification ;
  rdfs:label "Requested" ;
.
:involvesTimeClassification a owl:DatatypeProperty ;
  rdfs:comment "Every event should have a time classification. The time classifications may be planned, estimated, expected, actual or requested." ;
  rdfs:label "Has Time Classification" ;
  rdfs:domain :Event ;
  rdfs:range :TimeClassification ;
.

# Milestone

:Milestone
  a owl:Class ;
  rdfs:comment "Each Association Event should have a Milestone associated with it. At the moment, only Start and End are allowed milestones." ;
  rdfs:label "Milestone" ;
.
:involvesMilestone a owl:DatatypeProperty ;
  rdfs:comment "The milestone may be start or end." ;
  rdfs:label "Milestone" ;
  rdfs:domain :Event ;
  rdfs:range :Milestone ;
.
:End
  a :Milestone ;
  rdfs:label "End" ;
.
:Start
  a :Milestone ;
  rdfs:label "Start" ;
.

# Involves predicates

:involves
  a owl:ObjectProperty ;
  rdfs:comment "An Event has associations established with Digital Twins, Locations or Logistic Actors. The meaning of this association depends on the type of event and the its' milestone." ;
  rdfs:domain :Event ;
  rdfs:label "Involves" ;
  rdfs:range owl:Thing ;
.
:involvesBusinessIdentifier
  a owl:DatatypeProperty ;
  rdfs:comment "Identifier that can be used to refer to an external system the business transaction where the event is involved in (e.g., AWB / eFTI / voyage number (IMO0191))" ;
  rdfs:domain :Event ;
  rdfs:label "Involves Business Identifier" ;
  rdfs:range xsd:string ;
  skos:altLabel "IMO0191"
.
:involvesDigitalTwin
  a owl:ObjectProperty ;
  rdfs:label "Involves Digital Twin" ;
  rdfs:comment "Used for grouping -- do not instantiate" ;
  rdfs:domain :Event ;
  rdfs:range DigitalTwin:PhysicalObject ;
  rdfs:subPropertyOf :involves ;
.
:involvesLocation
  a owl:ObjectProperty ;
  rdfs:comment "This relation establishes an association between an Event and a Location. The exact meaning depends on the type of Event, which is inferred from this property and the second association the event has." ;
  rdfs:domain :Event ;
  rdfs:label "Involves Location" ;
  rdfs:range Location:BusinessLocation ;
.
:involvesActor
  a owl:ObjectProperty ;
  rdfs:label "Involves Actor" ;
  rdfs:comment "This relation establishes an association between an Event and an Actor." ;
  rdfs:domain :Event ;
  rdfs:range LegalPerson:Actor ;
  rdfs:subPropertyOf :involves ;
.
:involvesPackagingType
  a owl:DatatypeProperty ;
  rdfs:label "Involves Packaging Type" ;
  rdfs:comment "This property denotes the packaging invovled in the association of the product/goods with a package." ;
  rdfs:domain :CargoAssociation ;
  rdfs:range xsd:string ;
  skos:altLabel "IMO0029"
.
:involvesTimestamp
  a owl:DatatypeProperty ;
  rdfs:comment "The timestamp expressed as a date and time, alongside the timezone it is specified";
  rdfs:label "Timestamp";
  rdfs:range xsd:dateTime ;
  rdfs:subPropertyOf :involves ;
  skos:Ã¤ltLabel "IMO00748"
.
:involvesTransportMeans
  a owl:ObjectProperty ;
  rdfs:comment "This relation establishes an association between an Event and a Transport Means Digital Twin. The exact meaning depends on the type of Event and its' milestone" ;
  rdfs:domain :Event ;
  rdfs:label "Involves Transport Means" ;
  rdfs:range DigitalTwin:TransportMeans ;
  rdfs:subPropertyOf :involvesDigitalTwin ;
.