@prefix rdf: <http://www.w3.org/1999/02/22-rdf-syntax-ns#> .
@prefix rdfs: <http://www.w3.org/2000/01/rdf-schema#> .
@prefix owl: <http://www.w3.org/2002/07/owl#> .
@prefix dc: <http://purl.org/dc/elements/1.1/> .
@prefix dcterms: <http://purl.org/dc/terms/> .
@prefix event: <https://ontology.tno.nl/logistics/federated/Event#> .
@prefix state: <https://ontology.tno.nl/logistics/federated/State#> .
@prefix lr: <https://ontology.tno.nl/logistics/federated/LogisticRoles#> .
@prefix : <https://ontology.tno.nl/logistics/federated/InteractionPattern#> .

<https://ontology.tno.nl/logistics/federated/InteractionPattern>
  a owl:Ontology ;
  dc:creator "Thom van Gessel (TNO)" ;
  dcterms:description "First draft for an ontology that describes interaction patterns (choreographies) in logistics." ;
  dcterms:language "en" ;
  owl:versionIRI <https://ontology.tno.nl/logistics/federated/InteractionPatternv-0.1.0> ;
  owl:versionInfo "0.1.0" ;
.

:InteractionPattern
  a owl:Class ;
  rdfs:comment "An interaction pattern containing states, transitions, an initial state and final state(s)." ;
  rdfs:label "Interaction pattern" ;
.

:Transition
  a owl:Class ;
  rdfs:comment "A transition with a source and target state type, and a sender and recipient role." ;
  rdfs:label "State transition" ;
.

:EventType
  a owl:Class ;
  rdfs:comment "Any subclass of event:Event" ;
  rdfs:label "Event type" ;
  owl:equivalentClass [ a owl:Restriction ; #TO DO: add this also as SHACL constraint (an instance of :EventType must be a subclass of event:Event)
    owl:onProperty rdfs:subClassOf ;
    owl:hasValue event:Event ;
  ] ;
.

:StateType
  a owl:Class ;
  rdfs:comment "Any subclass of state:State" ;
  rdfs:label "State type" ;
  owl:equivalentClass [ a owl:Restriction ; #TO DO: add this also as SHACL constraint (an instance of :StateType must be a subclass of state:State)
    owl:onProperty rdfs:subClassOf ;
    owl:hasValue state:State ;
  ] ;
.

:transition
  a owl:ObjectProperty ;
  rdfs:comment "Indicates that a transition occurs in an interaction pattern." ;
  rdfs:label "Interaction pattern contains transition" ;
  rdfs:domain :InteractionPattern ;
  rdfs:range :Transition ;
.

:state
  a owl:ObjectProperty ;
  rdfs:comment "Indicates that a state occurs in an interaction pattern." ;
  rdfs:label "Interaction pattern contains state" ;
  rdfs:domain :InteractionPattern ;
  rdfs:range :StateType ;
.

:initialState
  a owl:ObjectProperty ;
  rdfs:subPropertyOf :state ;
  rdfs:comment "Indicates the initial state in an interaction pattern." ;
  rdfs:label "Interaction pattern has initial state" ;
  rdfs:domain :InteractionPattern ;
  rdfs:range :StateType ;
.

:finalState
  a owl:ObjectProperty ;
  rdfs:subPropertyOf :state ;
  rdfs:comment "Indicates a final state in an interaction pattern." ;
  rdfs:label "Interaction pattern has final state" ;
  rdfs:domain :InteractionPattern ;
  rdfs:range :StateType ;
.

:interaction
  a owl:ObjectProperty ;
  rdfs:comment "Connects a state transition to its corresponding event type." ;
  rdfs:label "has interaction" ;
  rdfs:domain :Transition ;
  rdfs:range :EventType ;
.

:source
  a owl:ObjectProperty ;
  rdfs:comment "Connects a state transition to its source state type." ;
  rdfs:label "has source state type" ;
  rdfs:domain :Transition ;
  rdfs:range :StateType ;
.

:target
  a owl:ObjectProperty ;
  rdfs:comment "Connects a state transition to its target state type." ;
  rdfs:label "has target state type" ;
  rdfs:domain :Transition ;
  rdfs:range :StateType ;
  skos:altLabel "IMO0281"
.

:senderRole
  a owl:ObjectProperty ;
  rdfs:comment "Connects a state transition to the role of its sender, typically lr:Customer or lr:LogisticServiceProvider." ;
  rdfs:label "has sender role" ;
  rdfs:domain :Transition ;
  rdfs:range lr:LogisticsRoles ;
.

:recipientRole
  a owl:ObjectProperty ;
  rdfs:comment "Connects a state transition to the role of its recipient, typically lr:Customer or lr:LogisticServiceProvider." ;
  rdfs:label "has recipient role" ;
  rdfs:domain :Transition ;
  rdfs:range lr:LogisticsRoles ;
.