@prefix : <https://ontology.tno.nl/logistics/federated/State#> .
@prefix rdfs: <http://www.w3.org/2000/01/rdf-schema#> .
@prefix owl: <http://www.w3.org/2002/07/owl#> .
@prefix dc: <http://purl.org/dc/elements/1.1/> .
@prefix dcterms: <http://purl.org/dc/terms/> .

<https://ontology.tno.nl/logistics/federated/State>
  a owl:Ontology ;
  dc:creator "Thom van Gessel (TNO)" ;
  dcterms:description "First draft for an ontology that describes states in logistics processes." ;
  dcterms:language "en" ;
  owl:versionIRI <https://ontology.tno.nl/logistics/federated/Statev-0.1.0> ;
  owl:versionInfo "0.1.0" ;
.

:State
  a owl:Class ;
  rdfs:comment "A state reflects a circumstance in a concrete logistics process." ;
  rdfs:label "State" ;
.
:AgreedOrderState
  a owl:Class ;
  rdfs:comment "A state in which agreement about a concrete order is reached." ;
  rdfs:label "Agreed order state" ;
  rdfs:subClassOf :State ;
.
:InExecutionState
  a owl:Class ;
  rdfs:comment "A state in which a concrete order is in execution." ;
  rdfs:label "In execution state" ;
  rdfs:subClassOf :State ;
.
:CompletedState
  a owl:Class ;
  rdfs:comment "A state in which a concrete order is completed." ;
  rdfs:label "Completed state" ;
  rdfs:subClassOf :State ;
.
:ToBeCancelledState
  a owl:Class ;
  rdfs:comment "A state in which a concrete order is to be cancelled." ;
  rdfs:label "To be cancelled state" ;
  rdfs:subClassOf :State ;
.